% \documentclass[fontsize=9pt,paper=letter,pagesize]{scrartcl} 
\documentclass[10pt,twoside]{book}

% Math notation stuff
\newcommand{\bldgr}[1]{{\mbox{\boldmath {${#1}$}}}} % Bold for lower-case Greek letters
\newcommand{\fat}[1]{\mathbf{#1}} % Bold for anything else
%\newcommand{\transp}{^\textrm{\small T}} % Transpose
\newcommand{\transp}{^T} % Transpose


\begin{document}

$$
\fat{y}( \fat{x}, \fat{w} )
= \fat{x} + \bldgr{\delta}( \fat{x}, \fat{w} )
$$

$$
t
$$

$$
y( x, t ) = x + t
$$

$$
E( t )
=
\sum_{n=1}^N
E_n( t ) 
$$

$$
E_n( t )
=
\left[ 
\mathcal{F}( x_n ) - \mathcal{M}( y( x_n, t ) )
\right]^2
$$

$$
E( t )
=
\sum_{n=1}^N
\left[ 
\mathcal{F}( x ) - \mathcal{M}( y( x_n, t ) )
\right]^2
$$

$$
\epsilon
$$

$$
\mathcal{M}( y( x_n, t+\epsilon ) ) 
\,\,
\simeq
\,\,
\mathcal{M}( y( x_n, t ) ) 
+ 
g_n \cdot \epsilon
$$

$$
g_n 
= 
\frac{\mathrm{d} \mathcal{M}( y( x_n, t ) ) }{\mathrm{d} y}
$$

$$
g_n 
= 
\frac{\mathrm{d} \mathcal{M}( y )}{\mathrm{d} y} \bigg|_{y=x_n+t}
$$

$$
E_n( t + \epsilon )
\,\,
=
\,\,
\left[ 
\mathcal{F}( x_n ) - \mathcal{M}( y( x_n, t + \epsilon ) )
\right]^2
$$

$$
\simeq
\,\,
\left[ 
\mathcal{F}( x_n ) - \mathcal{M}( y( x_n, t ) ) - g_n \cdot \epsilon
\right]^2
$$

$$
E( t + \epsilon )
=
\sum_{n=1}^N
E_n( t + \epsilon ) 
$$

$$
\tau_n = \mathcal{F}( x_n ) - \mathcal{M}( y( x_n, t ) )
$$

$$
\epsilon = ( \bldgr{\psi}^T \bldgr{\psi} )^{-1} \bldgr{\psi}^T \bldgr{\tau}
$$

$$
\bldgr{\psi} = ( g_1, \ldots, g_N )^T
$$

$$
\bldgr{\psi} 
= 
\left(
\begin{array}{c}
g_1 \\
\vdots \\
g_N
\end{array}
\right)
= 
%\mathrm{diag}( g_1, \ldots, g_N )
\left(
\begin{array}{ccc}
g_1 & & \\
& \ddots & \\
& & g_N
\end{array}
\right)
\left(
\begin{array}{c}
1 \\
\vdots \\
1
\end{array}
\right)
$$

$$
\underbrace{
\begin{array}{ccc}
\phantom{g_1} & \phantom{\cdots} & \phantom{g_N}
\end{array}
}_{\fat{G}}}
$$

$$
\bldgr{\tau} 
= 
\left(
\begin{array}{c}
\tau_1 \\
\vdots \\
\tau_N
\end{array}
\right)
$$

$$
\bldgr{\tau} 
= 
\left(
\begin{array}{c}
\mathcal{F}( x_1 ) - \mathcal{M}( y( x_1, t ) ) \\
\vdots \\
\mathcal{F}( x_N ) - \mathcal{M}( y( x_N, t ) )
\end{array}
\right)
$$

$$
D > 1
$$

$$
M > 1
$$

$$
t 
\,\,
\gets 
\,\,
t + \epsilon
$$

$$
\delta_1(\fat{x}, \fat{w}_1)
$$

$$
\delta_2(\fat{x}, \fat{w}_2)
$$


\end{document}



